src/program_proof/simplepb/simplelog/proof.v
@@ -11,14 +11,9 @@ From Goose.github_com.mit_pdos.gokv.simplepb Require Export simplelog.
 
 Section global_proof.
 
-Context {params:pbParams.t}.
-Import pbParams.
-Notation OpType := (Sm.OpType pb_record).
-Notation has_op_encoding := (Sm.has_op_encoding pb_record).
-Notation is_readonly_op := (Sm.is_readonly_op pb_record).
-Notation has_snap_encoding := (Sm.has_snap_encoding pb_record).
-Notation compute_reply := (Sm.compute_reply pb_record).
-Instance e : EqDecision OpType := (Sm.OpType_EqDecision pb_record).
+Context {sm_record:Sm.t}.
+Import Sm.
+Instance e : EqDecision OpType := OpType_EqDecision.
 
 Class simplelogG Σ := SimplelogG {
   simplelog_fmlistG :> fmlistG ((list OpType) * bool) Σ;
@@ -152,12 +147,7 @@ End global_proof.
 Section sm_defn.
 
 Context {sm_record:Sm.t}.
-Notation OpType := (Sm.OpType sm_record).
-Notation has_op_encoding := (Sm.has_op_encoding sm_record).
-Notation has_snap_encoding := (Sm.has_snap_encoding sm_record).
-Notation compute_reply := (Sm.compute_reply sm_record).
-Notation is_readonly_op := (Sm.is_readonly_op sm_record).
-Notation apply_postcond := (Sm.apply_postcond sm_record).
+Import Sm.
 
 Context `{!heapGS Σ}.
 Implicit Types own_InMemoryStateMachine : list OpType → iProp Σ.
@@ -247,13 +237,7 @@ Context `{!heapGS Σ}.
 
 Context {params:pbParams.t}.
 Import pbParams.
-Notation OpType := (Sm.OpType pb_record).
-Notation has_op_encoding := (Sm.has_op_encoding pb_record).
-Notation has_snap_encoding := (Sm.has_snap_encoding pb_record).
-Notation compute_reply := (Sm.compute_reply pb_record).
-Notation is_readonly_op := (Sm.is_readonly_op pb_record).
-Notation apply_postcond := (Sm.apply_postcond pb_record).
-
+Import Sm.
 
 Record simplelog_names :=
 {
